test-suite/bugChecker.v
@@ -6,21 +6,15 @@ Set Printing Universes.
 
 Definition T := Type.
 Definition T' := T.
-Definition foo' := (T : T').
+(* Definition foo' := (T : T'). *)
+Definition foo' := let T := Type in (T : T).
 
 Quote Recursively Definition p := foo'.
+(* Template Check foo'. *)
 Eval lazy in (let '(Σ, t) := decompose_program p ([], init_graph) in
+    (* infer_term Σ t). *)
 let t := (tSort (Universe.super (Level.Level "Top.10"))) in
 let u := (tSort (Universe.make (Level.Level "Top.10"))) in
 let Γ := [] in
-leq_term (snd Σ) t u).
+(* leq_term (snd Σ) t u). *)
 isconv (fst Σ) fuel (Cumul (snd Σ)) Γ t [] u []).
-
-
-    (*      convert_leq Σ [] (tSort (Universe.super (Level.Level "Top.10"))) *)
-    (*                  (tSort (Universe.make (Level.Level "Top.10")))). *)
-
-    (* infer Σ [] t). *)
-
-    (* let '(Σ, t) := decompose_program p ([], init_graph) in *)
-    (* check_wf_env Σ ;; infer_term Σ t. *)
