theories/Typing.v
@@ -563,22 +563,31 @@ with typing_spine (Σ : global_context) (Γ : context) : term -> list term -> te
     typing_spine Σ Γ (subst0 hd B) tl B' ->
     typing_spine Σ Γ T (cons hd tl) B'.
 
+
 Definition add_constraints_env u (Σ : global_context)
   := (fst Σ, add_constraints u (snd Σ)).
+
+Definition add_global_decl (decl : global_decl) (Σ : global_context) :=
+  let univs := match decl with
+               | ConstantDecl _ d => d.(cst_universes)
+               | InductiveDecl _ d => d.(ind_universes)
+               end
+  in (decl :: fst Σ, add_constraints univs (snd Σ)).
 
 Fixpoint decompose_program (p : program) (Σ : global_context) : global_context * term :=
   match p with
   | PConstr s u ty trm p =>
     let decl :=  {| cst_universes := u; cst_type := ty; cst_body := Some trm |} in
-    decompose_program p (ConstantDecl s decl :: fst Σ, add_constraints u (snd Σ))
+    decompose_program p (add_global_decl (ConstantDecl s decl) Σ)
   | PAxiom s u ty p =>
     let decl := {| cst_universes := u; cst_type := ty; cst_body := None |} in
-    decompose_program p (ConstantDecl s decl :: fst Σ, add_constraints u (snd Σ))
+    decompose_program p (add_global_decl (ConstantDecl s decl) Σ)
   | PType ind u m inds p =>
     let decl := {| ind_npars := m; ind_bodies := inds; ind_universes := u |} in
-    decompose_program p (InductiveDecl ind decl :: fst Σ, add_constraints u (snd Σ))
+    decompose_program p (add_global_decl (InductiveDecl ind decl) Σ)
   | PIn t => (Σ, t)
   end.
+
 
 Definition isType (Σ : global_context) (Γ : context) (t : term) :=
   { s : _ & Σ ;;; Γ |- t : tSort s }.
