translations/tsl_param2.v
@@ -93,7 +93,7 @@ with tsl_term  (fuel : nat) (Σ : global_context) (E : tsl_table) (Γ : context)
     | Some t => ret t
     | None => raise (TranslationNotFound (string_of_gref (ConstructRef i n)))
     end
-  | t => match infer Σ init_graph Γ t with
+  | t => match infer Σ Γ t with
         | Checked typ => let t1 := tsl_rec1 0 t in
                         t2 <- tsl_rec2 fuel Σ E Γ t ;;
                         let typ1 := tsl_rec1 0 typ in
@@ -173,14 +173,14 @@ Definition tsl_mind_decl (ΣE : tsl_context)
     + (* arity  *)
       refine (t2 <- tsl2' ind.(ind_type) ;;
               let i1 := tsl_rec1 0 (tInd (mkInd kn i) []) in
-              ret (try_reduce (fst ΣE) [] fuel (mkApp t2 i1))).
+              ret (try_reduce (fst (fst ΣE)) [] fuel (mkApp t2 i1))).
     + (* constructors *)
       refine (monad_map_i _ ind.(ind_ctors)).
       intros k ((name, typ), nargs).
       refine (t2 <- tsl2' typ ;;
               let t2 := fold_left_i (fun t i u => replace u i t) L t2 in
               let c1 := tsl_rec1 0 (tConstruct (mkInd kn i) k []) in
-              match reduce_opt RedFlags.default (fst ΣE) [] (* for debugging but we could use try_reduce *)
+              match reduce_opt RedFlags.default (fst (fst ΣE)) [] (* for debugging but we could use try_reduce *)
                                fuel (mkApp t2 c1) with
               | Some t' => ret (tsl_ident name, t', nargs)
               | None => raise TranslationNotHandeled
@@ -212,11 +212,11 @@ Notation "'El' A" := (sigma (π1 A) (π2 A)) (at level 20).
 
 Definition ty := nat -> nat.
 
-Run TemplateProgram (TslParam ([],[]) "nat" >>= print_nf).
+Run TemplateProgram (TslParam emptyTC "nat" >>= print_nf).
 
 Require Vector.
 Require Even.
-Run TemplateProgram (TslParam ([],[]) "list" >>= tmPrint).
+Run TemplateProgram (TslParam emptyTC "list" >>= tmPrint).
 Check (listᵗ : forall (A : TYPE), list A.1 -> Type).
 Check (nilᵗ : forall (A : TYPE), listᵗ A nil).
 Check (consᵗ : forall (A : TYPE) (x : El A) (lH : exists l, listᵗ A l),
